Refactors code. Still one admit

newio/DM.fst
@@ -8,6 +8,58 @@ open Free
 open Free.IO
 open Hist
 
+(** the behavior of f can differ based on the history in iio **)
+let rec trace_of (lt:trace) (m:io 'a) (x:'a) =
+  match lt, m with
+  | [], Return x' -> x == x'
+  | e::es, Call cmd arg k -> 
+     (let (| cmd', arg', res' |) = destruct_event e in 
+          (cmd' == cmd /\ arg == arg' /\ (trace_of es (k res') x)))
+  | _, _ -> False
+
+(** this is too complicated for io, but may be needed for iio: 
+let rec trace_of (lt:trace) (m:io 'a) (x:'a) =
+  match lt, m with
+  | [], Return x' -> x == x'
+  | [], Call cmd arg k -> (forall h. io_wps cmd arg (fun lt r -> lt == []) h) /\ (forall r. trace_of lt (k r) x)
+  | e::es, Call cmd arg k -> 
+          // either this is a silent call so we skip
+          ((forall h. io_wps cmd arg (fun lt r -> lt == []) h) /\ (forall r. trace_of lt (k r) x)) \/
+          // either this call has an event on the local trace
+          (let (| cmd', arg', res' |) = destruct_event e in 
+            (cmd' == cmd /\ arg == arg' /\ (trace_of es (k res') x)))
+  | _, _ -> False **)
+
+(** maybe worth thinking about a way to avoid using a different function: 
+let exact_2 x y = fun x' y' -> x == x' /\ y == y'
+
+let rec lemma_more_general_law m p h : 
+  Lemma 
+    (requires theta m p h) 
+    (ensures (forall lt x. theta m (exact_2 lt x) h ==> p lt x)) = () **)
+
+let exists_trace_of (x:'a) (m:io 'a) =
+  exists lt. trace_of lt m x
+
+let rec lemma_return_of_implies_exists_trace_of (x:'a) (m:io 'a) : 
+  Lemma
+    (requires (x `return_of` m))
+    (ensures (exists_trace_of x m)) =
+  match m with
+  | Return _ -> assert (trace_of [] m x)
+  | Call cmd arg k -> begin
+    eliminate exists r. (x `return_of` (k r)) returns (exists_trace_of x m) with _. begin
+      lemma_return_of_implies_exists_trace_of x (k r);
+      assert (exists klt. trace_of klt (k r) x) by (assumption ());
+      eliminate exists klt. trace_of klt (k r) x returns (exists_trace_of x m) with _. begin
+        let e = convert_call_to_event cmd arg r in
+        introduce exists lt. (trace_of lt m x) with (e::klt) and begin
+          assert (trace_of (e::klt) m x)
+        end
+      end
+    end
+  end
+
 (** Inspierd from Kenji's thesis (2.4.5) **)
 let rec theta #a
   (m : io a) : hist a =
@@ -15,13 +67,30 @@ let rec theta #a
   | Return x -> hist_return x
   | Call cmd arg k ->
     hist_bind (io_wps cmd arg) (fun r -> theta (k r))
+  
+let rec lemma_theta_result_implies_post m p h : 
+  Lemma 
+    (requires theta m p h) 
+    (ensures (forall x lt. trace_of lt m x ==> p lt x)) =
+  introduce forall x lt. trace_of lt m x ==> p lt x with begin
+    introduce trace_of lt m x ==> p lt x with _. begin
+      match m with
+      | Return _ -> ()
+      | Call cmd arg k -> begin
+        let e::klt = lt in
+        let (| cmd', arg', res' |) = destruct_event e in
+        lemma_theta_result_implies_post (k res') (hist_post_shift p [convert_call_to_event cmd arg res']) (convert_call_to_event cmd arg res' :: h);
+        assert (trace_of klt (k res') x);
+        assert (hist_post_shift p [convert_call_to_event cmd arg res'] klt x)
+      end
+    end
+  end
 
 let lemma_theta_is_monad_morphism_ret v h p :
-  Lemma
-    (theta (io_return v) == hist_return v) by (compute ()) = ()
+  Lemma (theta (io_return v) == hist_return v) by (compute ()) = ()
 
 (** TODO: remove the admits **)
-let rec lemma_theta_is_monad_morphism_bind (m:io 'a) (f:'a -> io 'b) :
+let rec lemma_theta_is_monad_morphism_bind (m:io 'a) (f:(x:'a) -> io 'b) :
   Lemma
     (theta (io_bind m f) == hist_bind (theta m) (fun x -> theta (f x))) = 
   match m with
@@ -81,7 +150,6 @@ let dm_bind
   Tot (dm b (hist_bind wp_v wp_f)) =
   admit ();
   lemma_theta_is_monad_morphism_bind v f;
-  (** hist is monotonic. **)
   io_bind v f
 
 let dm_subcomp (a:Type) (wp1 wp2: hist a) (f : dm a wp1) :
@@ -92,3 +160,12 @@ let dm_subcomp (a:Type) (wp1 wp2: hist a) (f : dm a wp1) :
 
 let dm_if_then_else (a : Type) (wp1 wp2: hist a) (f : dm a wp1) (g : dm a wp2) (b : bool) : Type =
   dm a (hist_if_then_else wp1 wp2 b)
+
+let lemma_hist_bind_implies_wp2_if_x
+  (wp1:hist 'a) (wp2:'a -> hist 'b)
+  (m:dm 'a wp1) p h x :
+  Lemma 
+    (requires (hist_bind wp1 wp2 p h /\ x `return_of` m))
+    (ensures (exists lt. wp2 x (hist_post_shift p lt) (List.rev lt @ h))) =
+  lemma_theta_result_implies_post m (fun lt r -> wp2 r (hist_post_shift p lt) (rev lt @ h)) h;
+  lemma_return_of_implies_exists_trace_of x m
