newio/DM7.fst
@@ -21,8 +21,6 @@ let get_fun #a #w (t : pdm a w) : Pure (dm a w) (requires get_pre t) (ensures fu
 let pdm_return (a:Type) (x:a) : pdm a (hist_return x) =
  (| True, (fun _ -> dm_return _ x) |)
 
-let hist_post_return (lt:trace) (x:'a) : hist_post 'a = fun lt' x' -> x == x' /\ lt == lt'
-
 (** this is to complicated for io, but may be needed for iio: 
 let rec trace_of (lt:trace) (m:io 'a) (x:'a) =
   match lt, m with
@@ -35,36 +33,6 @@ let rec trace_of (lt:trace) (m:io 'a) (x:'a) =
           (let (| cmd', arg', res' |) = destruct_event e in 
             (cmd' == cmd /\ arg == arg' /\ (trace_of es (k res') x)))
   | _, _ -> False **)
-let rec trace_of (lt:trace) (m:io 'a) (x:'a) =
-  match lt, m with
-  | [], Return x' -> x == x'
-  | e::es, Call cmd arg k -> 
-     (let (| cmd', arg', res' |) = destruct_event e in 
-          (cmd' == cmd /\ arg == arg' /\ (trace_of es (k res') x)))
-  | _, _ -> False
-
-(** the behavior of f can differ based on the history in iio **)
-let exists_trace_of (x:'a) (m:io 'a) =
-  exists lt. trace_of lt m x
-
-let rec lemma_return_of_implies_exists_trace_of (x:'a) (m:io 'a) : 
-  Lemma
-    (requires (x `return_of` m))
-    (ensures (exists_trace_of x m)) =
-  match m with
-  | Return _ -> assert (trace_of [] m x)
-  | Call cmd arg k -> begin
-    eliminate exists r. (x `return_of` (k r)) returns (exists_trace_of x m) with _. begin
-      lemma_return_of_implies_exists_trace_of x (k r);
-      assert (exists klt. trace_of klt (k r) x) by (assumption ());
-      eliminate exists klt. trace_of klt (k r) x returns (exists_trace_of x m) with _. begin
-        let e = convert_call_to_event cmd arg r in
-        introduce exists lt. (trace_of lt m x) with (e::klt) and begin
-          assert (trace_of (e::klt) m x)
-        end
-      end
-    end
-  end
 
 (** maybe worth thinking about a way to avoid using a different function: 
 let exact_2 x y = fun x' y' -> x == x' /\ y == y'
@@ -73,50 +41,22 @@ let rec lemma_more_general_law m p h :
   Lemma 
     (requires theta m p h) 
     (ensures (forall lt x. theta m (exact_2 lt x) h ==> p lt x)) = () **)
-  
-let rec lemma_theta_result_implies_post m p h : 
-  Lemma 
-    (requires theta m p h) 
-    (ensures (forall x lt. trace_of lt m x ==> p lt x)) =
-  introduce forall lt x. trace_of lt m x ==> p lt x with begin
-    introduce trace_of lt m x ==> p lt x with _. begin
-      match m with
-      | Return _ -> ()
-      | Call cmd arg k -> begin
-        let e::klt = lt in
-        let (| cmd', arg', res' |) = destruct_event e in
-        lemma_theta_result_implies_post (k res') (hist_post_shift p [convert_call_to_event cmd arg res']) (convert_call_to_event cmd arg res' :: h);
-        assert (trace_of klt (k res') x);
-        assert (hist_post_shift p [convert_call_to_event cmd arg res'] klt x)
-      end
-    end
-  end
 
-let lemma_hist_bind_implies_wp2_0
-  (wp1:hist 'a) (wp2:'a -> hist 'b)
-  (m:dm 'a wp1) 
-  p h x :
-  Lemma 
-    (requires (hist_bind wp1 wp2 p h /\ x `return_of` m))
-    (ensures (exists lt. wp2 x (fun lt' r' -> p (lt @ lt') r') (List.rev lt @ h))) =
-  lemma_theta_result_implies_post m (fun lt r -> wp2 r (fun lt' r' -> p (lt @ lt') r') (rev lt @ h)) h;
-  lemma_return_of_implies_exists_trace_of x m
-
-let lemma_hist_bind_implies_wp2
+let glue_lemma_hist_bind_implies_wp2_if_x
   (wp1:hist 'a) (wp2:'a -> hist 'b)
   (m:pdm 'a wp1) 
   p h x :
   Lemma 
     (requires (hist_bind wp1 wp2 p h /\ x `return_of` (get_fun m)))
-    (ensures (exists lt. wp2 x  (fun lt' r' -> p (lt @ lt') r') (List.rev lt @ h))) =
-  lemma_hist_bind_implies_wp2_0 wp1 wp2 (get_fun m) p h x
+    (ensures (exists lt. wp2 x  (hist_post_shift p lt) (List.rev lt @ h))) =
+  lemma_hist_bind_implies_wp2_if_x wp1 wp2 (get_fun m) p h x
 
 let pdm_bind (a b:Type)
   (wp1:hist a) (wp2:a -> hist b)
   (f:pdm a wp1) 
   (g:(x:a) -> pdm b (wp2 x)) :
   pdm b (hist_bind wp1 wp2) =
-  Classical.forall_intro_3 (Classical.move_requires_3 (lemma_hist_bind_implies_wp2 wp1 wp2 f));
+  Classical.forall_intro_3 (Classical.move_requires_3 (glue_lemma_hist_bind_implies_wp2_if_x wp1 wp2 f));
   (| (get_pre f /\ (forall x. x `return_of` (get_fun f) ==> get_pre (g x))), 
      (fun _ -> dm_bind a b wp1 wp2 (get_fun f) (fun x -> get_fun (g x))) 
    |)
@@ -127,7 +67,6 @@ let pdm_subcomp (a:Type) (wp1:hist a) (wp2:hist a) (f:pdm a wp1) :
     (ensures fun _ -> True) =
   (| get_pre f, (fun _ -> dm_subcomp a wp1 wp2 (get_fun f)) |)
 
-  
 unfold
 let pdm_if_then_else 
   (a : Type)
@@ -136,8 +75,7 @@ let pdm_if_then_else
   (f : pdm a wp1)
   (g : pdm a wp2)
   (b : bool) : Type =
-  pdm a
-    (hist_if_then_else wp1 wp2 b)
+  pdm a (hist_if_then_else wp1 wp2 b)
 
 total
 reifiable
@@ -160,17 +98,11 @@ effect IO
   IOwp a 
     (fun (p:hist_post a) (h:trace) -> pre h /\ (forall lt r. post h lt r ==>  p lt r)) 
 
-let lemma_another #a #event w :
-  Lemma (forall (p:hist_post #event a) h. wp_lift_pure_hist w p h ==> as_requires w) =
-    assert (forall (p:hist_post #event a) x. p [] x ==> True) ;
-    FStar.Monotonic.Pure.elim_pure_wp_monotonicity w ;
-    assert (forall (p:hist_post #event a). w (fun x -> p [] x) ==> w (fun _ -> True))
-
 let lift_pure_pdm (a : Type) 
   (w : pure_wp a)
   (f:(eqtype_as_type unit -> PURE a w)) : 
   pdm a (wp_lift_pure_hist w) =
-  lemma_another #a #event w;
+  lemma_wp_lift_pure_hist_implies_as_requires #a #event w;
   (| as_requires w, (fun _ -> 
     FStar.Monotonic.Pure.elim_pure_wp_monotonicity_forall ();
     let r = f () in
